theorem.v
@@ -12,9 +12,358 @@ Require Export typing.
 
 Require Export lemmas.
 
-
-Theorem Theoremone : forall S, exists gamma:environment, exists l:label, exists T:TracePat,
-(progTyping gamma l S T) -> 
-(memTraceObliv gamma S).
+(**
+Lemma labelequal_int : forall M1 M2 x l1 l2 n1 n2, (lowEquivalentMem M1 M2) ->
+(M1 x = Some (vint n1 l1)) -> (M2 x = Some (vint n2 l2)) -> 
+(l1 = l2).
 Proof.
+Admitted.
+**)
+
+Lemma lowEquiv_persist : forall M1 M2 x v, (lowEquivalentMem M1 M2) ->
+(lowEquivalentMem (memdefine M1 x v) (memdefine M2 x v)).
+Proof.
+intros M1 M2 x v H.
+unfold lowEquivalentMem.
+split.
+intros x0 v0.
+unfold memdefine.
+remember (varideq x0 x).
+destruct b.
+apply iff_refl.
+apply H.
+intros x0 v0.
+unfold memdefine.
+remember (varideq x0 x).
+destruct b.
+apply iff_refl.
+apply H.
+Qed.
+
+Lemma lowEquiv_sym : forall M1 M2, (lowEquivalentMem M1 M2) -> (lowEquivalentMem M2 M1).
+Proof.
+intros M1 M2 H.
+unfold lowEquivalentMem in *.
+split.
+intros x v.
+apply iff_sym.
+apply H.
+intros x v.
+apply iff_sym.
+apply H.
+Qed.
+
+Lemma lowEquiv_persist_high_int : forall M1 x v o, 
+(exists v1, M1 x = Some (vint v1 (o_high o))) ->
+(lowEquivalentMem (memdefine M1 x (vint v (o_high o))) M1).
+Proof.
+intros M1 x v o H.
+unfold lowEquivalentMem.
+split.
+intros x0 v0.
+unfold memdefine.
+remember (varideq x0 x).
+destruct b.
+split.
+intros HH.
+inversion HH.
+
+intros HH.
+unfold varideq in Heqb.
+destruct x0.
+destruct i.
+destruct x.
+destruct i.
+remember (beq_nat n n0).
+destruct b.
+symmetry in Heqb0.
+apply beq_nat_true in Heqb0.
+rewrite Heqb0 in HH.
+rewrite HH in H.
+inversion H.
+inversion H0.
+inversion Heqb.
+apply iff_refl.
+
+
+intros x0 v0.
+unfold memdefine.
+unfold varideq.
+destruct x0.
+destruct x.
+destruct i.
+destruct i0.
+remember (beq_nat n n0).
+destruct b.
+split.
+intros HH.
+inversion HH.
+intros HH.
+symmetry in Heqb.
+apply beq_nat_true in Heqb.
+rewrite Heqb in HH.
+rewrite HH in H.
+inversion H.
+inversion H0.
+apply iff_refl.
+Qed.
+
+Lemma lowEquiv_persist_high_arr : forall M1 x v o, 
+(exists v1, M1 x = Some (varr v1 (o_high o))) ->
+(lowEquivalentMem (memdefine M1 x (varr v (o_high o))) M1).
+Proof.
+intros M1 x v o H.
+unfold lowEquivalentMem.
+split.
+intros x0 v0.
+unfold memdefine.
+remember (varideq x0 x).
+destruct b.
+split.
+intros HH.
+inversion HH.
+
+intros HH.
+unfold varideq in Heqb.
+destruct x0.
+destruct i.
+destruct x.
+destruct i.
+remember (beq_nat n n0).
+destruct b.
+symmetry in Heqb0.
+apply beq_nat_true in Heqb0.
+rewrite Heqb0 in HH.
+rewrite HH in H.
+inversion H.
+inversion H0.
+inversion Heqb.
+apply iff_refl.
+
+
+intros x0 v0.
+unfold memdefine.
+unfold varideq.
+destruct x0.
+destruct x.
+destruct i.
+destruct i0.
+remember (beq_nat n n0).
+destruct b.
+split.
+intros HH.
+inversion HH.
+intros HH.
+symmetry in Heqb.
+apply beq_nat_true in Heqb.
+rewrite Heqb in HH.
+rewrite HH in H.
+inversion H.
+inversion H0.
+apply iff_refl.
+Qed.
+
+Lemma lowEquiv_trans : forall M1 M2 M3, (lowEquivalentMem M1 M2) -> 
+(lowEquivalentMem M2 M3) ->
+(lowEquivalentMem M1 M3).
+Proof.
+intros M1 M2 M3 H1 H2.
+unfold lowEquivalentMem in *.
+split.
+intros x v.
+apply iff_trans with (M2 x = Some (vint v low)).
+apply H1.
+apply H2.
+intros x v.
+apply iff_trans with (M2 x = Some (varr v low)).
+apply H1.
+apply H2.
+Qed.
+
+Lemma lowEquiv_refl : forall M, (lowEquivalentMem M M).
+Proof.
+intros M.
+unfold lowEquivalentMem.
+split.
+intros x v.
+apply iff_refl.
+intros x v.
+apply iff_refl.
+Qed.
+
+
+Theorem Theoremone : forall S (gamma:environment) (l:label) (T:TracePat),
+((progTyping gamma l S T) -> 
+(memTraceObliv gamma S)).
+Proof.
+intros S gamma l T.
+intros H.
+destruct H.
+induction s.
+(*epsilon case *)
+intros M1 M2 t1 M1' t2 M2'.
+intros HH1 HH4 HH5 HH2 HH3.
+inversion HH2.
+inversion H6.
+inversion HH3.
+inversion H16.
+split.
+apply equal_equiv.
+rewrite <- H20.
+rewrite <- H10.
+apply HH1.
+(*assign case Note, likely garbage past this point*)
+intros M1 M2 t1 M1' t2 M2'.
+intros HH1 HH2 HH3 HH4 HH5.
+inversion HH1. 
+inversion HH4.
+inversion H8.
+inversion HH5.
+inversion H22.
+inversion H.
+assert (t0 = t4).
+destruct l2.
+(**rewrite H25.
+rewrite H18.
+rewrite H11.
+rewrite H4.**)
+remember lemmasix.
+apply a with gamma e T0 M1 M2 t0 t4 n n0 in H36.
+inversion H36.
+apply H40.
+assumption.
+assumption.
+assumption.
+assumption.
+remember lemmaseven.
+apply e3 with gamma e o T0 M1 M2 t0 t4 n n0 in H36;
+repeat assumption.
+assert (l = l4).
+unfold gammavalid in HH2.
+assert (((gamma v = Some (lnat l)) <-> (exists n, M1 v = Some (vint n l))) /\(
+ (gamma v = Some (larr l)) <-> (exists n, M1 v = Some (varr n l)))).
+apply HH2.
+apply proj1 in H41.
+apply proj2 in H41.
+assert (gamma v = Some( lnat l)).
+apply H41.
+exists n1.
+assumption.
+assert (Some (lnat l4) = Some (lnat l)).
+rewrite <- H42.
+rewrite <- H38.
+reflexivity.
+inversion H43.
+reflexivity.
+rewrite <- H41 in *.
+assert (l = l1).
+unfold gammavalid in HH3.
+assert (((gamma v = Some (lnat l1)) <-> (exists n, M2 v = Some (vint n l1))) /\(
+ (gamma v = Some (larr l1)) <-> (exists n, M2 v = Some (varr n l1)))).
+apply HH3.
+apply proj1 in H42.
+apply proj2 in H42.
+assert (gamma v = Some( lnat l1)).
+apply H42.
+exists n2.
+assumption.
+assert (Some (lnat l1) = Some (lnat l)).
+rewrite <- H43.
+rewrite <- H38.
+reflexivity.
+inversion H44.
+reflexivity.
+rewrite <- H42 in *.
+rewrite H40 in *.
+destruct l.
+assert (l2 = low).
+inversion H39.
+unfold mtojoin in H44.
+destruct l0.
+symmetry.
+assumption.
+inversion H44.
+rewrite H43 in *.
+remember lemmasix.
+apply a with gamma e T0 M1 M2 t0 t4 n n0 in H36.
+inversion H36.
+rewrite H45.
+split.
+apply equal_equiv.
+apply lowEquiv_persist.
+assumption.
+assumption.
+assumption.
+rewrite H40.
+assumption.
+assumption.
+split.
+unfold evttrace.
+apply equal_equiv.
+apply lowEquiv_trans with M1.
+apply lowEquiv_persist_high_int.
+exists n1.
+apply H16.
+apply lowEquiv_trans with M2.
+assumption.
+apply lowEquiv_sym.
+apply lowEquiv_persist_high_int.
+exists n2.
+apply H30.
+
+
+.
+assert (gamma v = Some (lnat l)).
+
+apply HH2.
+
+
+destruct l4.
+rewrite H39.
+apply HH2.
+apply HH3.
+apply H14.
+apply H28.
+assert (t1 = t2).
+destruct l4.
+
+
+split.
+remember lemmasix.
+apply a with gamma e  T0 M1 M2 t0 t4 n n0 in H35 .
+inversion H35.
+rewrite H39.
+rewrite H40.
+assert (l=l1).
+apply labelequal_int with M1 M2 v n1 n2.
+apply HH1.
+apply H15.
+apply H29.
+rewrite H41.
+apply equal_equiv.
+apply HH2.
+apply HH3.
+apply H14.
+apply H28.
+apply 
+apply concat_decomp_equiv.
+apply equal_equiv.
+apply concat_decomp_equiv.
+apply equal_equiv.
+
+split.
+apply concat_decomp_equiv.
+apply equal_equiv.
+apply concat_decomp_equiv.
+assumption.
+
+simpl.
+intros M1.
+destruct H.
+admit.
+
+
+induction l0.
+inversion .
+intros H.
 Admitted.
